Add an AVL tree in the examples (#283)
* tests: add AVL example

Signed-off-by: Ryan Lahfa <ryan.lahfa@inria.fr>

* tests: add Lean formalization for AVL

Signed-off-by: Ryan Lahfa <ryan.lahfa@inria.fr>

* Fix minor extraction issues

* Start fixing the AVL tree example

* Commit some missing files

* Make a minor modification

* Update the code of the AVL tree

* Fix the code of the AVL tree

* Regenerate the code of the AVL tree

* Make progress on updating the proofs of the AVL trees

* Make progress on updating the proofs of the AVL tree

* Make minor modifications to the AVLs

* Move and update the code of the AVL tree

* Regenerate the Lean model for the AVL tree

* Generate simp lemmas for the custom field projectors

* Regenerate the types for the AVL test

* Make progress on the proof of the AVL tree

* Make progress on the proofs

* Make progress on the proofs of the AVL tree

* Make progress on the proofs of the AVL

* Cleanup a bit

* Cleanup a bit

* Do more cleanup

* Make progress on the AVL tree

* Make good progress on the avl

* Make minor modifications

* Fix pspec for mutually recursive functions

* Regenerate the test files

* Improve pspec and progress and cleanup a bit

* Add a comment

* Fix an issue with the CI and regenerate the tests

* Cleanup

* Do more cleanup

* Make progress generate warnings instead of errors if there are too many ids

* Fix a CI issue

* Fix a bug in destructure_abs

* Cleanup a bit

* Fix a minor issue in the flake.nix

---------

Signed-off-by: Ryan Lahfa <ryan.lahfa@inria.fr>
Co-authored-by: Ryan Lahfa <ryan.lahfa@inria.fr>

compiler/InterpreterBorrows.ml
@@ -1803,6 +1803,13 @@ let destructure_abs (span : Meta.span) (abs_kind : abs_kind) (can_end : bool)
                 let value =
                   ALoan (ASharedLoan (PNone, bids, sv, mk_aignored span ty))
                 in
+                (* We need to update the type of the value: abstract shared loans
+                   have the type `& ...` - TODO: this is annoying and not very clean... *)
+                let ty =
+                  (* Take the first region of the abstraction - this doesn't really matter *)
+                  let r = RegionId.Set.min_elt abs0.regions in
+                  TRef (RFVar r, ty, RShared)
+                in
                 { value; ty }
               in
               let avl = List.append [ av ] avl in
