tests/lean/Avl/Properties.lean
@@ -1,0 +1,1030 @@
+import Avl.Funs
+import Avl.Types
+import Avl.OrderSpec
+
+namespace avl
+
+open Primitives Result
+
+-- TODO: move
+@[simp]
+def Option.allP {α : Type u} (p : α → Prop) (x : Option α) : Prop :=
+  match x with
+  | none => true
+  | some x => p x
+
+abbrev Subtree (T : Type) := Option (Node T)
+
+mutual
+@[simp]
+def Node.height: Node T -> Nat
+| Node.mk y left right _ => 1 + max (Subtree.height left) (Subtree.height right)
+
+@[simp]
+def Subtree.height: Subtree T -> Nat
+| none => 0
+| some n => Node.height n
+end
+
+mutual
+@[simp]
+def Node.size: Node T -> Nat
+| Node.mk y left right _ => 1 + Subtree.size left + Subtree.size right
+
+@[simp]
+def Subtree.size: Subtree T -> Nat
+| none => 0
+| some n => 1 + Node.size n
+end
+
+def Tree.nil: Tree T := { root := none }
+
+-- Automatic synthesization of this seems possible at the Lean level?
+instance: Inhabited (Tree T) where
+  default := Tree.nil
+
+instance [Inhabited T]: Inhabited (Node T) where
+  default := ⟨ Inhabited.default, none, none, 0#i8 ⟩
+
+mutual
+@[simp, reducible] def Subtree.v (tree: Subtree T) : Set T :=
+  match tree with
+  | none => ∅
+  | some node => node.v
+
+@[simp, reducible] def Node.v (node : Node T) : Set T :=
+  match node with
+  | .mk x left right _ => {x} ∪ Subtree.v left ∪ Subtree.v right
+end
+
+@[reducible]
+def Tree.v (t: Tree T): Set T := Subtree.v t.root
+
+mutual
+@[simp] def Subtree.forall (p: Node T -> Prop) (st : Subtree T) : Prop :=
+  match st with
+  | none => true
+  | some st => st.forall p
+termination_by Subtree.size st
+decreasing_by simp_wf
+
+def Node.forall (p: Node T -> Prop) (node : Node T) : Prop :=
+  p node ∧
+  Subtree.forall p node.left ∧ Subtree.forall p node.right
+termination_by Node.size node
+decreasing_by all_goals (simp_wf; simp [Node.left, Node.right]; split <;> simp <;> scalar_tac)
+end
+
+@[simp]
+theorem Subtree.forall_left {p: Node T -> Prop} {t: Node T}: Node.forall p t -> Subtree.forall p t.left := by
+  cases t; simp_all [Node.forall]
+
+@[simp]
+theorem Subtree.forall_right {p: Node T -> Prop} {t: Node T}: Subtree.forall p t -> Subtree.forall p t.right := by
+  cases t; simp_all [Node.forall]
+
+mutual
+theorem Subtree.forall_imp {p q: Node T -> Prop} {t: Subtree T}: (∀ x, p x -> q x) -> Subtree.forall p t -> Subtree.forall q t
+  := by
+  match t with
+  | none => simp
+  | some node =>
+    simp
+    intros
+    apply @Node.forall_imp T p q <;> tauto
+
+theorem Node.forall_imp {p q: Node T -> Prop} {t: Node T}: (∀ x, p x -> q x) -> Node.forall p t -> Node.forall q t := by
+  match t with
+  | .mk x left right height =>
+    simp [Node.forall]
+    intros Himp Hleft Hright Hx
+    simp [*]
+    split_conjs <;> apply @Subtree.forall_imp T p q <;> tauto
+
+end
+
+def Node.balanceFactor (node : Node T) : ℤ :=
+  Subtree.height node.right - Subtree.height node.left
+
+def Subtree.balanceFactor (t: Subtree T): ℤ :=
+  match t with
+  | .none => 0
+  | .some x => x.balanceFactor
+
+@[simp]
+theorem Subtree.some_balanceFactor (t: Node T) :
+  Subtree.balanceFactor (some t) = t.balanceFactor := by
+  simp [balanceFactor]
+
+@[simp, reducible]
+def Node.invAuxNotBalanced [LinearOrder T] (node : Node T) : Prop :=
+  node.balance_factor.val = node.balanceFactor ∧
+  (∀ x ∈ Subtree.v node.left, x < node.value) ∧
+  (∀ x ∈ Subtree.v node.right, node.value < x)
+
+def Node.invAux [LinearOrder T] (node : Node T) : Prop :=
+  Node.invAuxNotBalanced node ∧
+  -1 ≤ node.balanceFactor ∧ node.balanceFactor ≤ 1
+
+@[reducible]
+def Node.inv [LinearOrder T] (node : Node T) : Prop :=
+  Node.forall Node.invAux node
+
+-- TODO: use a custom set
+@[aesop safe forward]
+theorem Node.inv_imp_current [LinearOrder T] {node : Node T} (hInv : node.inv) :
+  node.balance_factor.val = node.balanceFactor ∧
+  (∀ x ∈ Subtree.v node.left, x < node.value) ∧
+  (∀ x ∈ Subtree.v node.right, node.value < x) ∧
+  -1 ≤ node.balanceFactor ∧ node.balanceFactor ≤ 1 := by
+  simp_all [Node.inv, Node.forall, Node.invAux]
+
+@[reducible]
+def Subtree.inv [LinearOrder T] (st : Subtree T) : Prop :=
+  match st with
+  | none => true
+  | some node => node.inv
+
+@[simp]
+theorem Subtree.inv_some [LinearOrder T] (s : Node T) : Subtree.inv (some s) = s.inv := by
+  rfl
+
+@[reducible]
+def Tree.height (t : Tree T) := Subtree.height t.root
+
+@[reducible]
+def Tree.inv [LinearOrder T] (t : Tree T) : Prop := Subtree.inv t.root
+
+@[simp]
+theorem Node.inv_mk [LinearOrder T] (value : T) (left right : Option (Node T)) (bf : I8):
+  (Node.mk value left right bf).inv ↔
+  ((Node.mk value left right bf).invAux ∧
+   Subtree.inv left ∧ Subtree.inv right) := by
+  have : ∀ (n : Option (Node T)), Subtree.forall invAux n = Subtree.inv n := by
+    unfold Subtree.forall
+    simp [Subtree.inv]
+  constructor <;>
+  simp [*, Node.inv, Node.forall]
+
+@[simp]
+theorem Node.inv_left [LinearOrder T] {t: Node T}: t.inv -> Subtree.inv t.left := by
+  simp [Node.inv]
+  intro
+  cases t; simp_all
+
+@[simp]
+theorem Node.inv_right [LinearOrder T] {t: Node T}: t.inv -> Subtree.inv t.right := by
+  simp [Node.inv]
+  intro
+  cases t; simp_all
+
+theorem Node.inv_imp_balance_factor_eq [LinearOrder T] {t: Node T} (hInv : t.inv) :
+  t.balance_factor.val = t.balanceFactor := by
+  simp [inv, Node.forall, invAux] at hInv
+  cases t; simp_all
+
+@[simp]
+theorem Node.lt_imp_not_in_right [LinearOrder T] (node : Node T) (hInv : node.inv) (x : T)
+  (hLt : x < node.value) :
+  x ∉ Subtree.v node.right := by
+  have ⟨ _, _, h, _ ⟩ := Node.inv_imp_current hInv
+  intro hIn
+  have := h x hIn
+  have := lt_asymm this
+  tauto
+
+@[simp]
+theorem Node.lt_imp_not_in_left [LinearOrder T] (node : Node T) (hInv : node.inv) (x : T)
+  (hLt : node.value < x) :
+  x ∉ Subtree.v node.left := by
+  have ⟨ _, h, _, _ ⟩ := Node.inv_imp_current hInv
+  intro hIn
+  have := h x hIn
+  have := lt_asymm this
+  tauto
+
+@[simp]
+theorem Node.value_not_in_right [LinearOrder T] (node : Node T) (hInv : node.inv) :
+  node.value ∉ Subtree.v node.right := by
+  have ⟨ _, _, h, _ ⟩ := Node.inv_imp_current hInv
+  intro hIn
+  have := h node.value hIn
+  have := ne_of_lt this
+  tauto
+
+@[simp]
+theorem Node.value_not_in_left [LinearOrder T] (node : Node T) (hInv : node.inv) :
+  node.value ∉ Subtree.v node.left := by
+  have ⟨ _, h, _, _ ⟩ := Node.inv_imp_current hInv
+  intro hIn
+  have := h node.value hIn
+  have := ne_of_lt this
+  tauto
+
+@[pspec]
+theorem Tree.find_loop_spec
+  {T : Type} (OrdInst : Ord T)
+  [DecidableEq T] [LinOrd : LinearOrder T] [Ospec: OrdSpecLinearOrderEq OrdInst]
+  (value : T) (t : Subtree T) (hInv : Subtree.inv t) :
+  ∃ b, Tree.find_loop T OrdInst value t = ok b ∧
+  (b ↔ value ∈ Subtree.v t) := by
+  rewrite [find_loop]
+  match t with
+  | none => simp
+  | some (.mk v left right height) =>
+    dsimp only
+    have hCmp := Ospec.infallible -- TODO
+    progress keep Hordering as ⟨ ordering ⟩; clear hCmp
+    have hInvLeft := Node.inv_left hInv
+    have hInvRight := Node.inv_right hInv
+    cases ordering <;> dsimp only
+    . /- node.value < value -/
+      progress
+      have hNotIn := Node.lt_imp_not_in_left _ hInv
+      simp_all
+      intro; simp_all
+    . /- node.value = value -/
+      simp_all
+    . /- node.value > value -/
+      progress
+      have hNotIn := Node.lt_imp_not_in_right _ hInv
+      simp_all
+      intro; simp_all
+
+theorem Tree.find_spec
+  {T : Type} (OrdInst : Ord T)
+  [DecidableEq T] [LinOrd : LinearOrder T] [Ospec: OrdSpecLinearOrderEq OrdInst]
+  (t : Tree T) (value : T) (hInv : t.inv) :
+  ∃ b, Tree.find T OrdInst t value = ok b ∧
+  (b ↔ value ∈ t.v) := by
+  rw [find]
+  progress
+  simp [Tree.v]; assumption
+
+-- TODO: move
+set_option maxHeartbeats 5000000
+
+@[pspec]
+theorem Node.rotate_left_spec
+  {T : Type} [LinearOrder T]
+  (x z : T) (a b c : Option (Node T)) (bf_x bf_z : I8)
+  -- Invariants for the subtrees
+  (hInvA : Subtree.inv a)
+  (hInvZ : Node.inv ⟨ z, b, c, bf_z ⟩)
+  -- Invariant for the complete tree (but without the bounds on the balancing operation)
+  (hInvX : Node.invAuxNotBalanced ⟨ x, a, some ⟨ z, b, c, bf_z ⟩, bf_x ⟩)
+  -- The tree is not balanced
+  (hBfX : bf_x.val = 2)
+  -- Z has a positive balance factor
+  (hBfZ : 0 ≤ bf_z.val)
+  :
+  ∃ ntree, rotate_left T ⟨ x, a, none, bf_x ⟩ ⟨ z, b, c, bf_z ⟩ = ok ntree ∧
+  let tree : Node T := ⟨ x, a, some ⟨ z, b, c, bf_z ⟩, bf_x ⟩
+  -- We reestablished the invariant
+  Node.inv ntree ∧
+  -- The tree contains the nodes we expect
+  Node.v ntree = Node.v tree ∧
+  -- The height is the same as before. The original height is 2 + height b, and by
+  -- inserting an element (which produced subtree c) we got a new height of
+  -- 3 + height b; after the rotation we get back to 2 + height b.
+  Node.height ntree = 2 + Subtree.height b
+  := by
+  rw [rotate_left]
+  simp [core.mem.replace]
+  -- Some proofs common to both cases
+  -- Elements in the left subtree are < z
+  have : ∀ (y : T), (y = x ∨ y ∈ Subtree.v a) ∨ y ∈ Subtree.v b → y < z := by
+    simp [invAux] at hInvZ
+    intro y hIn
+    -- TODO: automate that
+    cases hIn
+    . rename _ => hIn
+      cases hIn
+      . simp [*]
+      . -- Proving: y ∈ a → y < z
+        -- Using: y < x ∧ x < z
+        rename _ => hIn
+        have hInv1 : y < x := by tauto
+        have hInv2 := hInvX.right.right z
+        simp at hInv2
+        apply lt_trans hInv1 hInv2
+    . tauto
+  -- Elements in the right subtree are < z
+  have : ∀ y ∈ Subtree.v c, z < y := by
+    simp [invAux] at hInvZ
+    tauto
+  -- Two cases depending on whether the BF of Z is 0 or 1
+  split
+  . -- BF(Z) == 0
+    simp at *
+    simp [*]
+    have hHeightEq : Subtree.height b = Subtree.height c := by
+      simp_all [balanceFactor, Node.invAux]
+      -- TODO: scalar_tac fails here (conversion int/nat)
+      omega
+    -- TODO: we shouldn't need this: scalar_tac should succeed
+    have : 1 + Subtree.height c = Subtree.height a + 2 := by
+      -- TODO: scalar_tac fails here (conversion int/nat)
+      simp_all [balanceFactor, Node.invAux]
+      omega
+    simp_all
+    split_conjs
+    . -- Partial invariant for the final tree starting at z
+      simp [Node.invAux, balanceFactor, *]
+      split_conjs <;> (try omega) <;> tauto
+    . -- Partial invariant for the subtree x
+      simp [Node.invAux, balanceFactor, *]
+      split_conjs <;> (try omega) <;> simp_all
+    . -- The sets are the same
+      apply Set.ext; simp; tauto
+    . -- The height didn't change
+      simp [balanceFactor] at *
+      replace hInvX := hInvX.left
+      simp_all
+      scalar_tac
+  . -- BF(Z) == 1
+    rename _ => hNotEq
+    simp at *
+    simp [*]
+    simp_all
+    have : bf_z.val = 1 := by
+      simp [Node.invAux] at hInvZ
+      omega
+    clear hNotEq hBfZ
+    have : Subtree.height c = 1 + Subtree.height b := by
+      simp [balanceFactor, Node.invAux] at *
+      replace hInvZ := hInvZ.left
+      omega
+    have : max (Subtree.height c) (Subtree.height b) = Subtree.height c := by
+      scalar_tac
+    -- TODO: we shouldn't need this: scalar_tac should succeed
+    have : Subtree.height c = 1 + Subtree.height a := by
+      -- TODO: scalar_tac fails here (conversion int/nat)
+      simp_all [balanceFactor, Node.invAux]
+      omega
+    have : Subtree.height a = Subtree.height b := by
+      simp_all
+    split_conjs
+    . -- Invariant for whole tree (starting at z)
+      simp [invAux, balanceFactor]
+      split_conjs <;> (try omega) <;> tauto
+    . -- Invariant for subtree x
+      simp [invAux, balanceFactor]
+      split_conjs <;> (try omega) <;> simp_all
+    . -- The sets are the same
+      apply Set.ext; simp; tauto
+    . -- The height didn't change
+      simp [balanceFactor] at *
+      replace hInvX := hInvX.left
+      simp_all
+      scalar_tac
+
+@[pspec]
+theorem Node.rotate_right_spec
+  {T : Type} [LinearOrder T]
+  (x z : T) (a b c : Option (Node T)) (bf_x bf_z : I8)
+  -- Invariants for the subtrees
+  (hInvC : Subtree.inv c)
+  (hInvZ : Node.inv ⟨ z, a, b, bf_z ⟩)
+  -- Invariant for the complete tree (but without the bounds on the balancing operation)
+  (hInvX : Node.invAuxNotBalanced ⟨ x, some ⟨ z, a, b, bf_z ⟩, c, bf_x ⟩)
+  -- The tree is not balanced
+  (hBfX : bf_x.val = -2)
+  -- Z has a positive balance factor
+  (hBfZ : bf_z.val ≤ 0)
+  :
+  ∃ ntree, rotate_right T ⟨ x, none, c, bf_x ⟩ ⟨ z, a, b, bf_z ⟩ = ok ntree ∧
+  let tree : Node T := ⟨ x, some ⟨ z, a, b, bf_z ⟩, c, bf_x ⟩
+  -- We reestablished the invariant
+  Node.inv ntree ∧
+  -- The tree contains the nodes we expect
+  Node.v ntree = Node.v tree ∧
+  -- The height is the same as before. The original height is 2 + height b, and by
+  -- inserting an element (which produced subtree c) we got a new height of
+  -- 3 + height b; after the rotation we get back to 2 + height b.
+  Node.height ntree = 2 + Subtree.height b
+  := by
+  rw [rotate_right]
+  simp [core.mem.replace]
+  -- Some proofs common to both cases
+  -- Elements in the right subtree are > z
+  have : ∀ (y : T), (y = x ∨ y ∈ Subtree.v b) ∨ y ∈ Subtree.v c → z < y := by
+    simp [invAux] at *
+    intro y hIn
+    -- TODO: automate that
+    cases hIn
+    . rename _ => hIn
+      cases hIn
+      . simp [*]
+      . tauto
+    . -- Proving: y ∈ c → z < y
+      -- Using: z < x ∧ x < y
+      have : z < x := by tauto
+      have : x < y := by tauto
+      apply lt_trans <;> tauto
+  -- Elements in the left subtree are < z
+  have : ∀ y ∈ Subtree.v a, y < z := by
+    simp_all [invAux]
+  -- Two cases depending on whether the BF of Z is 0 or 1
+  split
+  . -- BF(Z) == 0
+    simp at *
+    simp [*]
+    have hHeightEq : Subtree.height a = Subtree.height b := by
+      simp_all [balanceFactor, Node.invAux]
+      -- TODO: scalar_tac fails here (conversion int/nat)
+      omega
+    -- TODO: we shouldn't need this: scalar_tac should succeed
+    have : 1 + Subtree.height a = Subtree.height c + 2 := by
+      -- TODO: scalar_tac fails here (conversion int/nat)
+      simp_all [balanceFactor, Node.invAux]
+      omega
+    simp_all
+    split_conjs
+    . -- Partial invariant for the final tree starting at z
+      simp [Node.invAux, balanceFactor, *]
+      split_conjs <;> (try omega) <;> tauto
+    . -- Partial invariant for the subtree x
+      simp [Node.invAux, balanceFactor, *]
+      split_conjs <;> (try omega) <;> simp_all
+    . -- The sets are the same
+      apply Set.ext; simp; tauto
+    . -- The height didn't change
+      simp [balanceFactor] at *
+      replace hInvX := hInvX.left
+      simp_all
+      scalar_tac
+  . -- BF(Z) == -1
+    rename _ => hNotEq
+    simp at *
+    simp [*]
+    simp_all
+    have : bf_z.val = -1 := by
+      simp [Node.invAux] at hInvZ
+      omega
+    clear hNotEq hBfZ
+    have : Subtree.height a = 1 + Subtree.height b := by
+      simp [balanceFactor, Node.invAux] at *
+      replace hInvZ := hInvZ.left
+      omega
+    have : max (Subtree.height a) (Subtree.height b) = Subtree.height a := by
+      scalar_tac
+    -- TODO: we shouldn't need this: scalar_tac should succeed
+    have : Subtree.height a = 1 + Subtree.height c := by
+      -- TODO: scalar_tac fails here (conversion int/nat)
+      simp_all [balanceFactor, Node.invAux]
+      omega
+    have : Subtree.height c = Subtree.height b := by
+      simp_all
+    split_conjs
+    . -- Invariant for whole tree (starting at z)
+      simp [invAux, balanceFactor]
+      split_conjs <;> (try omega) <;> tauto
+    . -- Invariant for subtree x
+      simp [invAux, balanceFactor]
+      split_conjs <;> (try omega) <;> simp_all
+    . -- The sets are the same
+      apply Set.ext; simp; tauto
+    . -- The height didn't change
+      simp [balanceFactor] at *
+      replace hInvX := hInvX.left
+      simp_all
+      scalar_tac
+
+@[pspec]
+theorem Node.rotate_left_right_spec
+  {T : Type} [LinearOrder T]
+  (x y z : T) (bf_x bf_y bf_z : I8)
+  (a b t0 t1 : Option (Node T))
+  -- Invariants for the subtrees
+  (hInvX : Node.invAuxNotBalanced ⟨ x, some ⟨ z, t0, some ⟨ y, a, b, bf_y ⟩, bf_z ⟩, t1, bf_x ⟩)
+  (hInvZ : Node.inv ⟨ z, t0, some ⟨ y, a, b, bf_y ⟩, bf_z ⟩)
+  (hInv1 : Subtree.inv t1)
+  -- The tree is not balanced
+  (hBfX : bf_x.val = -2)
+  -- Z has a positive balance factor
+  (hBfZ : bf_z.val = 1)
+  :
+  let x_tree := ⟨ x, none, t1, bf_x ⟩
+  let y_tree := ⟨ y, a, b, bf_y ⟩
+  let z_tree := ⟨ z, t0, some y_tree, bf_z ⟩
+  let tree : Node T := ⟨ x, some z_tree, t1, bf_x ⟩
+  ∃ ntree, rotate_left_right T x_tree z_tree = ok ntree ∧
+  -- We reestablished the invariant
+  Node.inv ntree ∧
+  -- The tree contains the nodes we expect
+  Node.v ntree = Node.v tree ∧
+  -- The height is the same as before. The original height is 2 + height a, and by
+  -- inserting an element (which produced subtree c) we got a new height of
+  -- 3 + height b; after the rotation we get back to 2 + height b.
+  Node.height ntree = 2 + Subtree.height t0
+  := by
+  intro x_tree y_tree z_tree tree
+  simp [rotate_left_right] -- TODO: this inlines the local decls
+  -- Some facts about the heights and the balance factors
+  -- TODO: automate that
+  have : Node.height z_tree = Subtree.height t1 + 2 := by
+    simp [y_tree, z_tree, inv, invAux, balanceFactor] at *; omega
+  have : Node.height y_tree = Subtree.height t0 + 1 := by
+    simp [y_tree, z_tree, inv, invAux, balanceFactor] at *; omega
+  have : bf_y.val + Subtree.height a = Subtree.height b := by
+    simp [y_tree, z_tree, inv, invAux, balanceFactor] at *; omega
+  simp [x_tree, y_tree, z_tree] at *
+  -- TODO: automate the < proofs
+  -- Auxiliary proofs for invAux for y
+  have : ∀ (e : T), (e = z ∨ e ∈ Subtree.v t0) ∨ e ∈ Subtree.v a → e < y := by
+    intro e hIn
+    simp [invAux] at *
+    cases hIn
+    . rename _ => hIn
+      -- TODO: those cases are cumbersome
+      cases hIn
+      . simp_all
+      . have : e < z := by tauto
+        have : z < y := by tauto
+        apply lt_trans <;> tauto
+    . tauto
+  have : ∀ (e : T), (e = x ∨ e ∈ Subtree.v b) ∨ e ∈ Subtree.v t1 → y < e := by
+    intro e hIn; simp [invAux] at *
+    cases hIn
+    . rename _ => hIn
+      cases hIn
+      . simp_all
+      . tauto
+    . have : y < x := by
+        replace hInvX := hInvX.right.left y
+        tauto
+      have : x < e := by tauto
+      apply lt_trans <;> tauto
+  -- Auxiliary proofs for invAux for z
+  have : ∀ e ∈ Subtree.v t0, e < z := by
+    intro x hIn; simp [invAux] at *
+    tauto
+  have : ∀ e ∈ Subtree.v a, z < e := by
+    intro e hIn; simp [invAux] at *
+    replace hInvZ := hInvZ.right.right.left e
+    tauto
+  -- Auxiliary proofs for invAux for x
+  have : ∀ e ∈ Subtree.v b, e < x := by
+    intro e hIn; simp [invAux] at *
+    replace hInvX := hInvX.right.left e
+    tauto
+  have : ∀ e ∈ Subtree.v t1, x < e := by
+    intro e hIn; simp [invAux] at *
+    tauto
+  -- Case disjunction on the balance factor of Y
+  split
+  . -- BF(Y) = 0
+    simp [balanceFactor] at *
+    split_conjs <;> (try simp [Node.invAux, balanceFactor, *])
+    . -- invAux for y
+      split_conjs <;> (try omega) <;> (try tauto)
+    . -- invAux for z
+      split_conjs <;> (try scalar_tac) <;> tauto
+    . -- invAux for x
+      split_conjs <;> (try scalar_tac) <;> tauto
+    . -- The sets are the same
+      apply Set.ext; simp [tree, z_tree, y_tree]; tauto
+    . -- Height
+      scalar_tac
+  . split <;> simp
+    . -- BF(Y) < 0
+      have : bf_y.val = -1 := by simp [Node.invAux] at *; omega
+      simp [balanceFactor] at *
+      split_conjs <;> (try simp [Node.invAux, balanceFactor, *])
+      . -- invAux for y
+        split_conjs <;> (try omega) <;> (try tauto)
+      . -- invAux for z
+        split_conjs <;> (try scalar_tac) <;> tauto
+      . -- invAux for x
+        split_conjs <;> (try scalar_tac) <;> tauto
+      . -- The sets are the same
+        apply Set.ext; simp [tree, z_tree, y_tree]; tauto
+      . -- Height
+        scalar_tac
+    . -- BF(Y) > 0
+      have : bf_y.val = 1 := by simp [Node.invAux] at *; omega
+      split_conjs <;> (try simp [Node.invAux, balanceFactor, *])
+      . -- invAux for y
+        split_conjs <;> (try omega) <;> (try tauto)
+      . -- invAux for z
+        split_conjs <;> (try scalar_tac) <;> tauto
+      . -- invAux for x
+        split_conjs <;> (try scalar_tac) <;> tauto
+      . -- The sets are the same
+        apply Set.ext; simp [tree, z_tree, y_tree]; tauto
+      . -- Height
+        scalar_tac
+
+@[pspec]
+theorem Node.rotate_right_left_spec
+  {T : Type} [LinearOrder T]
+  (x y z : T) (bf_x bf_y bf_z : I8)
+  (a b t0 t1 : Option (Node T))
+  -- Invariants for the subtrees
+  (hInvX : Node.invAuxNotBalanced ⟨ x, t1, some ⟨ z, some ⟨ y, b, a, bf_y ⟩, t0, bf_z ⟩, bf_x ⟩)
+  (hInvZ : Node.inv ⟨ z, some ⟨ y, b, a, bf_y ⟩, t0, bf_z ⟩)
+  (hInv1 : Subtree.inv t1)
+  -- The tree is not balanced
+  (hBfX : bf_x.val = 2)
+  -- Z has a negative balance factor
+  (hBfZ : bf_z.val = -1)
+  :
+  let x_tree := ⟨ x, t1, none, bf_x ⟩
+  let y_tree := ⟨ y, b, a, bf_y ⟩
+  let z_tree := ⟨ z, some y_tree, t0, bf_z ⟩
+  let tree : Node T := ⟨ x, t1, some z_tree, bf_x ⟩
+  ∃ ntree, rotate_right_left T x_tree z_tree = ok ntree ∧
+  -- We reestablished the invariant
+  Node.inv ntree ∧
+  -- The tree contains the nodes we expect
+  Node.v ntree = Node.v tree ∧
+  -- The height is the same as before. The original height is 2 + height b, and by
+  -- inserting an element (which produced subtree c) we got a new height of
+  -- 3 + height b; after the rotation we get back to 2 + height b.
+  Node.height ntree = 2 + Subtree.height t1
+  := by
+  intro x_tree y_tree z_tree tree
+  simp [rotate_right_left] -- TODO: this inlines the local decls
+  -- Some facts about the heights and the balance factors
+  -- TODO: automate that
+  have : Node.height z_tree = Subtree.height t1 + 2 := by
+    simp [y_tree, z_tree, inv, invAux, balanceFactor] at *; omega
+  have : Node.height y_tree = Subtree.height t0 + 1 := by
+    simp [y_tree, z_tree, inv, invAux, balanceFactor] at *; omega
+  have : bf_y.val + Subtree.height b = Subtree.height a := by
+    simp [y_tree, z_tree, inv, invAux, balanceFactor] at *; omega
+  simp [x_tree, y_tree, z_tree] at *
+  -- TODO: automate the < proofs
+  -- Auxiliary proofs for invAux for y
+  have : ∀ (e : T), (e = z ∨ e ∈ Subtree.v a) ∨ e ∈ Subtree.v t0 → y < e := by
+    intro e hIn
+    simp [invAux] at *
+    cases hIn
+    . rename _ => hIn
+      -- TODO: those cases are cumbersome
+      cases hIn
+      . simp_all
+      . tauto
+    . have : z < e := by tauto
+      have : y < z := by tauto
+      apply lt_trans <;> tauto
+  have : ∀ (e : T), (e = x ∨ e ∈ Subtree.v t1) ∨ e ∈ Subtree.v b → e < y := by
+    intro e hIn; simp [invAux] at *
+    cases hIn
+    . rename _ => hIn
+      cases hIn
+      . simp_all
+      . have : x < y := by
+          replace hInvX := hInvX.right.right y
+          tauto
+        have : e < x := by tauto
+        apply lt_trans <;> tauto
+    . tauto
+  -- Auxiliary proofs for invAux for z
+  have : ∀ e ∈ Subtree.v t0, z < e := by
+    intro x hIn; simp [invAux] at *
+    tauto
+  have : ∀ e ∈ Subtree.v a, e < z := by
+    intro e hIn; simp [invAux] at *
+    replace hInvZ := hInvZ.right.left e
+    tauto
+  -- Auxiliary proofs for invAux for x
+  have : ∀ e ∈ Subtree.v b, x < e := by
+    intro e hIn; simp [invAux] at *
+    replace hInvX := hInvX.right.right e
+    tauto
+  have : ∀ e ∈ Subtree.v t1, e < x := by
+    intro e hIn; simp [invAux] at *
+    tauto
+  -- Case disjunction on the balance factor of Y
+  split
+  . -- BF(Y) = 0
+    simp [balanceFactor] at *
+    split_conjs <;> (try simp [Node.invAux, balanceFactor, *])
+    . -- invAux for y
+      split_conjs <;> (try omega) <;> (try tauto)
+    . -- invAux for z
+      split_conjs <;> (try scalar_tac) <;> tauto
+    . -- invAux for x
+      split_conjs <;> (try scalar_tac) <;> tauto
+    . -- The sets are the same
+      apply Set.ext; simp [tree, z_tree, y_tree]; tauto
+    . -- Height
+      scalar_tac
+  . split <;> simp
+    . -- BF(Y) > 0
+      have : bf_y.val = 1 := by simp [Node.invAux] at *; omega
+      simp [balanceFactor] at *
+      split_conjs <;> (try simp [Node.invAux, balanceFactor, *])
+      . -- invAux for y
+        split_conjs <;> (try omega) <;> (try tauto)
+      . -- invAux for z
+        split_conjs <;> (try scalar_tac) <;> tauto
+      . -- invAux for x
+        split_conjs <;> (try scalar_tac) <;> tauto
+      . -- The sets are the same
+        apply Set.ext; simp [tree, z_tree, y_tree]; tauto
+      . -- Height
+        scalar_tac
+    . -- BF(Y) < 0
+      have : bf_y.val = -1 := by simp [Node.invAux] at *; omega
+      split_conjs <;> (try simp [Node.invAux, balanceFactor, *])
+      . -- invAux for y
+        split_conjs <;> (try omega) <;> (try tauto)
+      . -- invAux for z
+        split_conjs <;> (try scalar_tac) <;> tauto
+      . -- invAux for x
+        split_conjs <;> (try scalar_tac) <;> tauto
+      . -- The sets are the same
+        apply Set.ext; simp [tree, z_tree, y_tree]; tauto
+      . -- Height
+        scalar_tac
+
+-- This rewriting lemma is problematic below
+attribute [-simp] Bool.exists_bool
+
+-- For the proofs of termination
+@[simp]
+theorem Node.left_height_lt_height (n : Node T) :
+  Subtree.height n.left < n.height := by
+  cases n; simp; scalar_tac
+
+@[simp]
+theorem Node.right_height_lt_height (n : Node T) :
+  Subtree.height n.right < n.height := by
+  cases n; simp; scalar_tac
+
+mutual
+
+@[pspec]
+theorem Node.insert_spec
+  {T : Type} (OrdInst : Ord T) [LinOrd : LinearOrder T] [Ospec: OrdSpecLinearOrderEq OrdInst]
+  (node : Node T) (value : T)
+  (hInv : Node.inv node) :
+  ∃ b node', Node.insert T OrdInst node value = ok (b, node') ∧
+  Node.inv node' ∧
+  Node.v node' = Node.v node ∪ {value} ∧
+  (if b then node'.height = node.height + 1 else node'.height = node.height) ∧
+  -- This is important for some of the proofs
+  (b → node'.balanceFactor ≠ 0) := by
+  rw [Node.insert]
+  have hCmp := Ospec.infallible -- TODO
+  progress as ⟨ ordering ⟩
+  split <;> rename _ => hEq <;> clear hCmp <;> simp at *
+  . -- value < node.value
+    progress as ⟨ updt, node', h1, h2 ⟩
+    simp_all
+  . -- value = node.value
+    cases node; simp_all
+  . -- node.value < value
+    progress as ⟨ updt, node', h1, h2 ⟩
+    simp_all
+termination_by (node.height, 1)
+decreasing_by all_goals simp_wf
+
+@[pspec]
+theorem Tree.insert_in_opt_node_spec
+  {T : Type} (OrdInst : Ord T) [LinOrd : LinearOrder T] [Ospec: OrdSpecLinearOrderEq OrdInst]
+  (tree : Option (Node T)) (value : T)
+  (hInv : Subtree.inv tree) :
+  ∃ b tree', Tree.insert_in_opt_node T OrdInst tree value = ok (b, tree') ∧
+  Subtree.inv tree' ∧
+  Subtree.v tree' = Subtree.v tree ∪ {value} ∧
+  (if b then Subtree.height tree' = Subtree.height tree + 1
+   else Subtree.height tree' = Subtree.height tree) ∧
+  (b → Subtree.height tree > 0 → Subtree.balanceFactor tree' ≠ 0) := by
+  rw [Tree.insert_in_opt_node]
+  cases hNode : tree <;> simp [hNode]
+  . -- tree = none
+    split_conjs
+    . simp [Node.invAux, Node.balanceFactor]
+    . simp [Subtree.inv]
+    . apply Set.ext; simp
+  . -- tree = some
+    rename Node T => node
+    have hNodeInv : Node.inv node := by simp_all
+    progress as ⟨ updt, tree' ⟩
+    simp_all
+termination_by (Subtree.height tree, 2)
+decreasing_by simp_wf; simp [*]
+
+-- TODO: any modification triggers the replay of the whole proof
+@[pspec]
+theorem Node.insert_in_left_spec
+  {T : Type} (OrdInst : Ord T)
+  [LinOrd : LinearOrder T] [Ospec: OrdSpecLinearOrderEq OrdInst]
+  (node : Node T) (value : T)
+  (hInv : Node.inv node)
+  (hLt : value < node.value) :
+  ∃ b node', Node.insert_in_left T OrdInst node value = ok (b, node') ∧
+  Node.inv node' ∧
+  Node.v node' = Node.v node ∪ {value} ∧
+  (if b then node'.height = node.height + 1 else node'.height = node.height) ∧
+  (b → node'.balanceFactor ≠ 0) := by
+  rw [Node.insert_in_left]
+  have hInvLeft : Subtree.inv node.left := by cases node; simp_all
+  progress as ⟨ updt, left_opt' .. ⟩
+  split
+  . -- the height of the subtree changed
+    have hBalanceFactor : node.balance_factor = node.balanceFactor ∧
+           -1 ≤ node.balanceFactor ∧ node.balanceFactor ≤ 1 := by
+      cases node; simp_all [Node.invAux]
+    progress as ⟨ i .. ⟩
+    split
+    . -- i = -2
+      simp
+      cases h: left_opt' with
+      | none => simp_all -- absurd
+      | some left' =>
+        simp [h]
+        cases node with | mk x left right balance_factor =>
+        split
+        . -- rotate_right
+          -- TODO: fix progress
+          cases h:left' with | mk z a b bf_z =>
+          progress as ⟨ tree', hInv', hTree'Set, hTree'Height ⟩
+          -- TODO: syntax for preconditions
+          . simp_all
+          . simp_all
+          . simp_all [Node.inv, Node.invAux, Node.invAuxNotBalanced, Node.balanceFactor]
+            scalar_tac
+          . simp_all
+          . -- End of the proof
+            simp [*]
+            split_conjs
+            . -- set reasoning
+              simp_all
+              apply Set.ext; simp
+              intro x; tauto
+            . -- height
+              simp_all [Node.invAux, Node.balanceFactor]
+              -- This assertion is not necessary for the proof, but it is important that it holds.
+              -- We can prove it because of the post-conditions `b → node'.balanceFactor ≠ 0` (see above)
+              have : bf_z.val = -1 := by scalar_tac
+              scalar_tac
+        . -- rotate_left_right
+          simp
+          cases h:left' with | mk z t0 y bf_z =>
+          cases h: y with
+          | none =>
+            -- Can't get there
+            simp_all [Node.balanceFactor, Node.invAux]
+          | some y =>
+            cases h: y with | mk y a b bf_y =>
+            progress as ⟨ tree', hInv', hTree'Set, hTree'Height ⟩
+            -- TODO: syntax for preconditions
+            . simp_all [Node.inv, Node.invAux, Node.invAuxNotBalanced, Node.balanceFactor]; scalar_tac
+            . simp_all
+            . simp_all
+            . simp_all [Node.invAux, Node.balanceFactor]; scalar_tac
+            . -- End of the proof
+              simp [*]
+              split_conjs
+              . apply Set.ext; simp_all
+                intro x; tauto
+              . simp_all [Node.invAux, Node.balanceFactor]
+                scalar_tac
+    . -- i ≠ -2: the height of the tree did not change
+      simp [*]
+      split_conjs
+      . cases node; simp_all [Node.invAux, Node.balanceFactor]
+        split_conjs <;> scalar_tac
+      . apply Set.ext; simp
+        cases node; simp_all
+        tauto
+      . simp_all
+        cases node with | mk node_value left right balance_factor =>
+        split <;> simp [Node.balanceFactor] at * <;> scalar_tac
+      . simp_all [Node.balanceFactor]
+        scalar_tac
+  . -- the height of the subtree did not change
+    simp [*]
+    split_conjs
+    . cases node;
+      simp_all [Node.invAux, Node.balanceFactor]
+    . apply Set.ext; simp; intro x
+      cases node; simp_all
+      tauto
+    . simp_all
+      cases node; simp_all
+termination_by (node.height, 0)
+decreasing_by simp_wf
+
+@[pspec]
+theorem Node.insert_in_right_spec
+  {T : Type} (OrdInst : Ord T)
+  [LinOrd : LinearOrder T] [Ospec: OrdSpecLinearOrderEq OrdInst]
+  (node : Node T) (value : T)
+  (hInv : Node.inv node)
+  (hGt : value > node.value) :
+  ∃ b node', Node.insert_in_right T OrdInst node value = ok (b, node') ∧
+  Node.inv node' ∧
+  Node.v node' = Node.v node ∪ {value} ∧
+  (if b then node'.height = node.height + 1 else node'.height = node.height) ∧
+  (b → node'.balanceFactor ≠ 0) := by
+  rw [Node.insert_in_right]
+  have hInvLeft : Subtree.inv node.right := by cases node; simp_all
+  progress as ⟨ updt, right_opt' .. ⟩
+  split
+  . -- the height of the subtree changed
+    have hBalanceFactor : node.balance_factor = node.balanceFactor ∧
+           -1 ≤ node.balanceFactor ∧ node.balanceFactor ≤ 1 := by
+      cases node; simp_all [Node.invAux]
+    progress as ⟨ i .. ⟩
+    split
+    . -- i = 2
+      simp
+      cases h: right_opt' with
+      | none => simp_all -- absurd
+      | some right' =>
+        simp [h]
+        split
+        . -- rotate_left
+          cases node with | mk x a right balance_factor =>
+          -- TODO: fix progress
+          cases h:right' with | mk z b c bf_z =>
+          progress as ⟨ tree', hInv', hTree'Set, hTree'Height ⟩
+          -- TODO: syntax for preconditions
+          . simp_all
+          . simp_all
+          . simp_all [Node.inv, Node.invAux, Node.invAuxNotBalanced, Node.balanceFactor]; scalar_tac
+          . simp_all
+          . -- End of the proof
+            simp [*]
+            split_conjs
+            . -- set reasoning
+              simp_all
+            . -- height
+              simp_all [Node.invAux, Node.balanceFactor]
+              -- This assertion is not necessary for the proof, but it is important that it holds.
+              -- We can prove it because of the post-conditions `b → node'.balanceFactor ≠ 0` (see above)
+              have : bf_z.val = 1 := by scalar_tac
+              scalar_tac
+        . -- rotate_right_left
+          cases node with | mk x t1 right balance_factor =>
+          simp
+          cases h:right' with | mk z y t0 bf_z =>
+          cases h: y with
+          | none =>
+            -- Can't get there
+            simp_all [Node.balanceFactor, Node.invAux]
+          | some y =>
+            cases h: y with | mk y b a bf_y =>
+            progress as ⟨ tree', hInv', hTree'Set, hTree'Height ⟩
+            -- TODO: syntax for preconditions
+            . simp_all [Node.inv, Node.invAux, Node.invAuxNotBalanced, Node.balanceFactor]; scalar_tac
+            . simp_all
+            . simp_all
+            . simp_all [Node.invAux, Node.balanceFactor]; scalar_tac
+            . -- End of the proof
+              simp [*]
+              split_conjs
+              . apply Set.ext; simp_all
+              . simp_all [Node.invAux, Node.balanceFactor]
+                scalar_tac
+    . -- i ≠ -2: the height of the tree did not change
+      simp [*]
+      split_conjs
+      . cases node; simp_all [Node.invAux, Node.balanceFactor]
+        split_conjs <;> scalar_tac
+      . apply Set.ext; simp
+        cases node; simp_all
+      . simp_all
+        cases node with | mk node_value left right balance_factor =>
+        split <;> simp [Node.balanceFactor] at * <;> scalar_tac
+      . simp_all [Node.balanceFactor]
+        scalar_tac
+  . -- the height of the subtree did not change
+    simp [*] -- TODO: annoying to use this simp everytime: put this in progress
+    split_conjs
+    . cases node;
+      simp_all [Node.invAux, Node.balanceFactor]
+    . apply Set.ext; simp; intro x
+      cases node; simp_all
+    . simp_all
+      cases node; simp_all
+termination_by (node.height, 0)
+decreasing_by simp_wf
+
+end
+
+@[pspec]
+theorem Tree.insert_spec {T : Type}
+  (OrdInst : Ord T) [LinOrd : LinearOrder T] [Ospec: OrdSpecLinearOrderEq OrdInst]
+  (tree : Tree T) (value : T)
+  (hInv : tree.inv) :
+  ∃ updt tree', Tree.insert T OrdInst tree value = ok (updt, tree') ∧
+  tree'.inv ∧
+  (if updt then tree'.height = tree.height + 1 else tree'.height = tree.height) ∧
+  tree'.v = tree.v ∪ {value} := by
+  rw [Tree.insert]
+  progress as ⟨ updt, tree' ⟩
+  simp [*]
+
+@[pspec]
+theorem Tree.new_spec {T : Type} (OrdInst : Ord T) :
+  ∃ t, Tree.new T OrdInst = ok t ∧ t.v = ∅ ∧ t.height = 0 := by
+  simp [new, Tree.v, Tree.height]
+
+end avl
